src/study/Nemonuri.Study.CSharpSyntaxRewriter2.Modifier/Nemonuri.StratifiedNode.NodeTheory.Descendant.fst
@@ -28,7 +28,7 @@ let rec get_count
       sum_for_get_count #t #lv #sn (
         select_in_children sn (
           fun psn csn -> (
-            lemma_child_node_level_is_lower_than_parent psn csn;
+            //lemma_child_node_level_is_lower_than_parent psn csn;
             get_count csn <: nat
           )
         )
@@ -43,7 +43,7 @@ let rec exists_in_descendant_or_self
     else
       exists_in_children sn (
         fun psn csn -> (
-          lemma_child_node_level_is_lower_than_parent psn csn;
+          //lemma_child_node_level_is_lower_than_parent psn csn;
           exists_in_descendant_or_self csn predicate
         )
       )
